modélisation Isabelle/sync-mod/SyncModProof.thy
@@ -21,6 +21,29 @@ proof (rule+)
     show "x st = 0"
     proof -
         *)
+lemma sending : assumes run:"HORun (HOMachine_to_Algorithm (k_mod.SyncMod_HOMachine k)) rho HO" (is "HORun ?A rho HO")
+assumes "(HOrcvdMsgs ?A p (HO (Suc r) p) (rho r)) q = Content (Val v)" (is "?msgs q = _")
+shows "\<exists>s. rho r q = Active s \<and> x s = v"
+proof (cases "rho r q")
+    case Aslept
+    hence "?msgs q = (if q \<in> HO (Suc r) p then Bot else Void)" using HOrcvdMsgs_def[of ?A p "HO (Suc r) p" "rho r"] by auto
+    thus "\<exists>s. rho r q = Active s \<and> x s = v" using \<open>?msgs q = Content (Val v)\<close> by auto
+next
+    case (Active sq)
+    have "sendMsg ?A q p sq = Val (x sq)" using HOrcvdMsgs_def[of ?A p "HO (Suc r) p" "rho r"] \<open>?msgs q = Content (Val v)\<close>
+        by (simp add: Active HOMachine_to_Algorithm_def k_mod.SyncMod_HOMachine_def k_mod.SyncMod_sendMsg_def)
+    hence "k_mod.SyncMod_sendMsg k q p sq = Val (x sq)"
+        using HOMachine_to_Algorithm_def k_mod.SyncMod_HOMachine_def by 
+        (simp add: \<open>\<And>k. k_mod.SyncMod_HOMachine k \<equiv> \<lparr>CinitState = \<lambda>p st crd. k_mod.SyncMod_initState k p st,
+        sendMsg = k_mod.SyncMod_sendMsg k, CnextState = \<lambda>p st msgs crd. k_mod.SyncMod_nextState k p st msgs,
+        HOcommPerRd = k_mod.SyncMod_commPerRd, HOcommGlobal = k_mod.SyncMod_commGlobal,
+        HOcommSchedule = k_mod.SyncMod_commSchedule\<rparr>\<close>)
+    hence "?msgs q = Content (Val (x sq))" using HOrcvdMsgs_def[of ?A p "HO (Suc r) p" "rho r"] \<open>?msgs q = Content (Val v)\<close>
+        by (simp add: Active \<open>sendMsg (HOMachine_to_Algorithm (k_mod.SyncMod_HOMachine k)) q p sq = Val (x sq)\<close>)
+    hence "rho r q = Active sq \<and> x sq = v"
+        using \<open>rho r q = Active sq\<close> \<open>?msgs q = Content (Val v)\<close> k_mod.SyncMod_sendMsg_def[of k q p sq] by auto
+    thus "\<exists>s. rho r q = Active s \<and> x s = v"  by auto
+qed
 
 lemma transition : assumes s_def:"rho r p = Active s"
 and ss_def:"rho (Suc r) p = Active ss"
@@ -56,114 +79,6 @@ proof -
         using \<open>x s  = k\<close> by auto
 qed
 
-lemma A1 : assumes run:"HORun (HOMachine_to_Algorithm (k_mod.SyncMod_HOMachine k)) rho HO" (is "HORun ?A _ _")
-and "k > 2"
-shows "\<forall>r v p s ss. rho r p = Active s \<longrightarrow> rho (Suc r) p = Active ss \<longrightarrow> x ss = v \<longrightarrow> 0 \<le> v \<and> v < k"
-proof (rule allI)+
-    fix r v s ss p
-    show "rho r p = Active s \<longrightarrow> rho (Suc r) p = Active ss \<longrightarrow> x ss = v \<longrightarrow> 0 \<le> v \<and> v < k"
-    proof (induction r arbitrary:p v s ss)
-        case 0
-        show ?case
-        proof (rule impI)+
-            assume s_def:"rho 0 p = Active s"
-            assume ss_def:"rho (Suc 0) p = Active ss"
-            assume "x ss = v"
-            have no_content:"\<forall>v q. HOrcvdMsgs ?A p (HO 1 p) (rho 0) q \<noteq> Content (Val v)" (is "\<forall>v q. ?msgs q \<noteq> _")
-            proof (rule allI)+
-                fix v
-                fix q
-                show "?msgs q \<noteq> Content (Val v)"
-                proof (cases "rho 0 q")
-                    case "Aslept"
-                    hence "?msgs q = (if q \<in> HO 1 p then Bot else Void)" using HOrcvdMsgs_def[of ?A p "HO 1 p" "rho 0"] by auto
-                    thus "?msgs q \<noteq> Content (Val v)" by auto
-                next
-                    case (Active sq)
-                    hence "?msgs q = (if q \<in> HO 1 p then Content Nope else Void)"
-                        using stating[of 0 rho q k HO sq] run by auto
-                    thus "?msgs q \<noteq> Content (Val v)" by auto
-                qed
-            qed
-            hence "\<forall>v. \<not> k_mod.concordant ?msgs v" by (simp add: k_mod.concordant_def)
-            moreover have "k_mod.SyncMod_nextState k p s ?msgs ss"
-                using transition[of rho 0 p s ss k HO] s_def ss_def run  by auto
-            ultimately have v_possible:"if k_mod.ready_force k ?msgs s then x ss = k - 1 else if x ss = 0 then True else False" 
-            using k_mod.SyncMod_nextState_def[of k p s ?msgs ss] by fastforce
-            show "0 \<le> v \<and> v < k"
-            proof (cases "k_mod.ready_force k ?msgs s") 
-                case True
-                thus "0 \<le> v \<and> v < k" using v_possible \<open>x ss = v\<close> by (meson no_content k_mod.ready_force_def)
-            next
-                case False
-                hence "v = 0" using v_possible \<open>x ss = v\<close> by simp
-                thus "0 \<le> v \<and> v < k" using \<open>k > 2\<close> by auto
-            qed
-        qed
-    next
-        case (Suc r)
-        fix p
-        show "rho (Suc r) p = Active s \<longrightarrow> rho (Suc (Suc r)) p = Active ss \<longrightarrow> x ss = v \<longrightarrow> 0 \<le> v \<and> v < k"
-        proof (rule impI)+
-            assume "rho (Suc r) p = Active s"
-            assume "rho (Suc (Suc r)) p = Active ss"
-            assume "x ss = v"
-            have "\<forall>q vv. HOrcvdMsgs ?A p (HO (Suc (Suc r)) p) (rho (Suc r)) q = Content (Val vv) \<longrightarrow> 0 \<le> vv \<and> vv < k"
-                (is "\<forall>q vv. ?msgs q = _ \<longrightarrow> _")
-            proof (rule allI impI)+
-                fix q :: Proc
-                fix vv
-                assume "?msgs q = Content (Val vv)"
-                show "0 \<le> vv \<and> vv < k"
-                proof (cases "rho (Suc r) q")
-                    case Aslept
-                    hence "?msgs q = (if q \<in> HO (Suc (Suc r)) p then Bot else Void)"
-                        using HOrcvdMsgs_def[of ?A p "HO (Suc (Suc r)) p" "rho (Suc r)"] by auto
-                    thus "0 \<le> vv \<and> vv < k" using \<open>?msgs q = Content (Val vv)\<close> by auto
-                next
-                    case (Active sq)
-                    show "0 \<le> vv \<and> vv < k"
-                    proof (cases "rho r q")
-                        case Aslept
-                        hence "?msgs q = (if q \<in> HO (Suc r) p then Content Nope else Void)"
-                            using run stating[of "Suc r" rho q k HO sq] \<open>rho (Suc r) q = Active sq\<close>
-                            \<open>?msgs q = Content (Val vv)\<close> by auto
-                        thus "0 \<le> vv \<and> vv < k" using \<open>?msgs q = Content (Val vv)\<close> by auto
-                    next
-                        case (Active sqq)
-                        have "sendMsg ?A q p sq = Val vv"
-                            using HOrcvdMsgs_def[of ?A p "HO (Suc (Suc r)) p" "rho (Suc r)"] \<open>?msgs q = Content (Val vv)\<close>
-                            \<open>rho (Suc r) q = Active sq\<close> by auto
-                        hence "x sq = vv" using HOMachine_to_Algorithm_def k_mod.SyncMod_HOMachine_def by 
-                            (simp add: \<open>\<And>k. k_mod.SyncMod_HOMachine k \<equiv> \<lparr>CinitState = \<lambda>p st crd. k_mod.SyncMod_initState k p st,
-                            sendMsg = k_mod.SyncMod_sendMsg k,
-                            CnextState = \<lambda>p st msgs crd. k_mod.SyncMod_nextState k p st msgs,
-                            HOcommPerRd = k_mod.SyncMod_commPerRd, HOcommGlobal = k_mod.SyncMod_commGlobal,
-                            HOcommSchedule = k_mod.SyncMod_commSchedule\<rparr>\<close>
-                            k_mod.SyncMod_sendMsg_def)
-                        thus "0 \<le> vv \<and> vv < k"
-                            using Suc.IH[of q sqq sq] \<open>rho r q = Active sqq\<close> \<open>rho (Suc r) q = Active sq\<close> by auto
-                    qed
-                qed
-            qed
-
-            have trans:"k_mod.SyncMod_nextState k p s ?msgs ss"
-                using run \<open>rho (Suc r) p = Active s\<close> \<open>rho (Suc (Suc r)) p = Active ss\<close> transition by auto
-            thus "0 \<le> v \<and> v < k"
-            proof (cases "k_mod.ready_force k ?msgs s")
-                case True
-                hence "x ss = k - 1" using trans k_mod.SyncMod_nextState_def by auto
-                thus "0 \<le> v \<and> v < k" using \<open>x ss = v\<close> \<open>k > 2\<close> by auto
-            next
-                case non_force:False
-                show "0 \<le> v \<and> v < k"
-                proof (cases "x ss = 0")
-                    case True
-                    thus "0 \<le> v \<and> v < k" using \<open>x ss = v\<close> \<open>k > 2\<close> by auto
-                next
-                    case False
-                    hence "\<exists>q. ?msgs q = Content (Val ((x ss - 1) mod k))"
-                        using trans k_mod.concordant_def k_mod.SyncMod_nextState_def[of k p s ?msgs ss] non_force by auto
 
 
 lemma A2 : assumes "k_mod.xi_nek HO xi"
@@ -205,15 +120,55 @@ proof -
             hence "k_mod.SyncMod_nextState k p ss ?msgs st"
                 using HOMachine_to_Algorithm_def k_mod.SyncMod_HOMachine_def[of k]
                 by (simp add: k_mod.simp_nextState)
-            ultimately have "k_mod.concordant ?msgs ((x st - 1) mod k)"
+            ultimately have "k_mod.concordant ?msgs ((x st - 1) mod k)" and "(x st) mod k = x st"
                 using k_mod.SyncMod_nextState_def[of k p ss ?msgs st] \<open>x st \<noteq> 0\<close> 
                 by auto
-            hence "\<forall>vv. ?msgs xi = Content (Val vv) \<longrightarrow> vv = ((x st - 1) mod k)" 
+            hence "\<forall>vv. ?msgs xi = Content (Val vv) \<longrightarrow> vv = ((x st - 1) mod k)"
                 using k_mod.concordant_def[of ?msgs "(x st - 1) mod k"] by auto
             hence "k - 1 = (x st - 1) mod k"
                 using \<open>?msgs xi = Content (Val (x s))\<close> \<open>x s = k - 1\<close> by auto
-            hence "0 = x st" by 
-            hence "\<exists>tem. ?msgs tem = Content (Val (x st)) \<and> (\<forall>q vv. ?msgs q = Content (Val vv) \<longrightarrow> vv = (x st))"
-                using k_mod.concordant_def[of ?msgs] by auto
+            hence "(x st) mod k = 0"  using \<open>(x st) mod k = x st\<close>
+                by (smt SendVal.distinct(1) \<open>k_mod.SyncMod_sendMsg k xi p s = Val (x s)\<close>
+                add_diff_inverse_nat add_le_cancel_left
+                assms(4) diff_is_0_eq k_mod.SyncMod_sendMsg_def le_add_diff_inverse linorder_not_less
+                mod_by_1 mod_if mod_less_divisor mod_less_eq_dividend nat_code(2))
+            thus "False" using \<open>(x st) mod k = x st\<close> \<open>x st \<noteq> 0\<close> by auto
+        qed
+    qed
+    thus "monovalent rho 0 r" using monovalent_def[of rho 0 r] by auto
+qed
 
-end
+lemma A3 : assumes "k_mod.xi_nek HO xi"
+and run:"HORun (HOMachine_to_Algorithm (k_mod.SyncMod_HOMachine k)) rho HO" (is "HORun ?A _ _")
+and "rho r xi = Active s"
+and "x s = k - 1"
+and "k > 2"
+and "monovalent rho v r"
+shows "monovalent rho (v+i) (r+i)"
+proof (induction i)
+    from assms(6) show \<open>monovalent rho (v+0) (r+0)\<close> by auto
+next
+    case (Suc i)
+    have "rho (r+i) xi \<noteq> Aslept"
+        using run HORun_def assms(3) nonAsleepAgain[of rho r xi ?A HO _ i] by (simp add: HORun_def add.commute)
+    then obtain sx where "rho (r+i) xi = Active sx" by (cases "rho (r+i) xi") auto
+    moreover have "rho (Suc (r+i)) xi \<noteq> Aslept"
+        using run HORun_def assms(3) nonAsleepAgain[of rho r xi ?A HO _ "i+1"] by (simp add: HORun_def add.commute)
+    then obtain sxx where "rho (Suc (r+i)) xi = Active sxx" by (cases "rho (Suc (r+i)) xi") auto
+    ultimately have "x sxx = v+i" using Suc.IH monovalent_def[of rho "v+i" "r+i" ] by auto
+    have "\<forall>p ss st. rho (r+Suc i) p = Active ss \<longrightarrow> rho (Suc (r+Suc i)) p = Active st \<longrightarrow> x st = v"
+    proof (rule+)
+        fix p ss st
+        assume "rho (r+Suc i) p = Active ss" and "rho (Suc (r+Suc i)) p = Active st"
+        hence "k_mod.SyncMod_nextState k p ss (HOrcvdMsgs ?A p (HO (Suc (r+Suc i)) p) (rho (r+Suc i))) st"
+            (is "k_mod.SyncMod_nextState k p ss ?msgs st") using run by (simp add:transition)
+        show "x st = v"
+        proof (cases "k_mod.ready_force k ?msgs ss")
+            case True
+            hence "\<exists>p1 p2 v1 v2. ?msgs p1 = Content (Val v1) \<and> ?msgs p2 = Content (Val v2) \<and> v1 \<noteq> v2"
+                using k_mod.ready_force_def by blast
+            then obtain p1 p2 v1 v2 where "?msgs p1 = Content (Val v1)" and "?msgs p2 = Content (Val v2)" and "v1 \<noteq> v2" by auto
+            then obtain s1 s2 where "rho (r+Suc i) p1 = Active s1 \<and> x s1 = v1" and "rho (r+Suc i) p2 = Active s2 \<and> x s2 = v2"
+                using run sending[of k rho HO p "r+Suc i" p1 v1] sending[of k rho HO p "r+Suc i" p2 v2] by auto
+            hence ""
+    show "monovalent rho (v+Suc i) (r+Suc i)"
